Logic/Propositional/Structural.lean
@@ -1,0 +1,59 @@
+namespace Logic.Propositional.Structural
+
+variable {Propn : Type}
+
+inductive Ctx
+  | nil
+  | cons (Γ : Ctx) (A : Propn)
+
+local notation "Ctx" => Ctx (Propn := Propn)
+
+inductive Hyp : (Γ : Ctx) → (A : Propn) → Type
+  | here : Hyp (.cons Γ A) A
+  | there (u : Hyp Γ A) : Hyp (Γ.cons B) A
+
+local notation "Hyp" => Hyp (Propn := Propn)
+
+def Subst (J : (Γ : Ctx) → (A : Propn) → Type) (Γ Γ' : Ctx) : Type :=
+  ∀ ⦃A⦄, (u : Hyp Γ A) → J Γ' A
+
+local notation "Subst" => Subst (Propn := Propn)
+
+def Subst.id : Subst Hyp Γ Γ
+  | _, u => u
+
+def Subst.weakening : Subst Hyp Γ (Γ.cons A)
+  | _ => .there
+
+def Subst.exchange : Subst Hyp (Ctx.cons Γ A |>.cons B) (Γ.cons B |>.cons A)
+  | _, .here => .there .here
+  | _, .there .here => .here
+  | _, .there (.there u) => u.there.there
+
+class JudgeTrans (J J' : (Γ : Ctx) → (A : Propn) → Type) where
+  transform (D : J Γ A) : J' Γ A
+
+local notation "JudgeTrans" => JudgeTrans (Propn := Propn)
+
+instance JudgeTrans.id : JudgeTrans J J where
+  transform D := D
+
+def Subst.mk [jt : JudgeTrans Hyp J] (D : J Γ A) : Subst J (Γ.cons A) Γ
+  | _, .here => D
+  | _, .there u => jt.transform u
+
+def Subst.map (jt : JudgeTrans J J') (γ : Subst J Γ Γ') : Subst J' Γ Γ'
+  | _, u => jt.transform (γ u)
+
+class Judge (J) extends JudgeTrans Hyp J where
+  rename (γ : Subst Hyp Γ Γ') {A} (D : J Γ A) : J Γ' A
+
+instance Hyp.judge : Judge Hyp where
+  rename γ := @γ
+
+def Subst.weaken [j : Judge J] (γ : Subst J Γ Γ') : Subst J Γ (Γ'.cons A)
+  | _, u => j.rename .weakening (γ u)
+
+def Subst.lift [j : Judge J] (γ : Subst J Γ Γ') : Subst J (Γ.cons A) (Γ'.cons A)
+  | _, .here => j.transform .here
+  | _, .there u => γ.weaken u
